theories/designs/utp_des_prog.thy
@@ -326,13 +326,13 @@ proof (induct n)
 next
   case (Suc n) note hyp = this
   have "(p \<turnstile>\<^sub>n Q) ;; (p \<turnstile>\<^sub>n Q) \<^bold>^ Suc n = (p \<turnstile>\<^sub>n Q) ;; (p \<turnstile>\<^sub>n Q) ;; (p \<turnstile>\<^sub>n Q) \<^bold>^ n"
-    by (simp)
+    by (simp add: upred_semiring.power_Suc)
   also have "... = (p \<turnstile>\<^sub>n Q) ;; ((\<Squnion> i \<in> {0..n} \<bullet> Q \<^bold>^ i wp p) \<turnstile>\<^sub>n Q \<^bold>^ Suc n)"
     by (simp add: hyp)
   also have "... = (p \<and> Q wp (\<Squnion> i \<in> {0..n} \<bullet> Q \<^bold>^ i wp p)) \<turnstile>\<^sub>n (Q ;; Q) ;; Q \<^bold>^ n"
-    by (simp add: ndesign_composition_wp seqr_assoc)
+    by (simp add: upred_semiring.power_Suc ndesign_composition_wp seqr_assoc)
   also have "... = (p \<and> (\<Squnion> i \<in> {0..n} \<bullet> Q \<^bold>^ Suc i wp p)) \<turnstile>\<^sub>n (Q ;; Q) ;; Q \<^bold>^ n"
-    by (simp add: wp)
+    by (simp add: upred_semiring.power_Suc wp)
   also have "... = (p \<and> (\<Squnion> i \<in> {0..n}. Q \<^bold>^ Suc i wp p)) \<turnstile>\<^sub>n (Q ;; Q) ;; Q \<^bold>^ n"
     by (simp add: USUP_as_Inf_image)
   also have "... = (p \<and> (\<Squnion> i \<in> {1..Suc n}. Q \<^bold>^ i wp p)) \<turnstile>\<^sub>n (Q ;; Q) ;; Q \<^bold>^ n"
@@ -342,7 +342,7 @@ next
   also have "... = ((\<Squnion> i \<in> {0..Suc n}. Q \<^bold>^ i wp p)) \<turnstile>\<^sub>n (Q ;; Q) ;; Q \<^bold>^ n"
     by (simp add: Iic_Suc_eq_insert_0 atLeast0AtMost conj_upred_def image_Suc_atMost)      
   also have "... = (\<Squnion> i \<in> {0..Suc n} \<bullet> Q \<^bold>^ i wp p) \<turnstile>\<^sub>n Q \<^bold>^ Suc (Suc n)"
-    by (simp add: USUP_as_Inf_image upred_semiring.mult_assoc)
+    by (simp add: upred_semiring.power_Suc USUP_as_Inf_image upred_semiring.mult_assoc)
   finally show ?case .
 qed
 
